proof/invariant-abstract/Invariants_AI.thy
@@ -1158,14 +1158,6 @@ lemma obj_at_get_object_True:
   unfolding obj_in_ta_def
   by force
 
-abbreviation ta_obj_upd :: "machine_word \<Rightarrow> kernel_object \<Rightarrow> machine_state \<Rightarrow> machine_state"
-  where
-  "ta_obj_upd p ko ms \<equiv> machine_state.touched_addresses_update ((\<union>) (obj_range p ko)) ms"
-
-abbreviation ms_ta_obj_upd :: "machine_word \<Rightarrow> kernel_object \<Rightarrow> 'a state \<Rightarrow> 'a state"
-  where
-  "ms_ta_obj_upd p ko s \<equiv> s \<lparr> machine_state := ta_obj_upd p ko (machine_state s) \<rparr>"
-
 lemma ko_at_tcb_at:
   "ko_at (TCB t) p s \<Longrightarrow> tcb_at p s"
   by (simp add: obj_at_def is_tcb)
