spec/machine/RISCV64/MachineOps.thy
@@ -75,11 +75,11 @@ definition
 
 definition
   clearTouchedAddresses :: "unit machine_monad"
-  where "clearTouchedAddresses \<equiv> modify (\<lambda>s. s\<lparr>touched_addresses := {}\<rparr>)"
+  where "clearTouchedAddresses \<equiv> modify (touched_addresses_update (\<lambda>_. {}))"
 
 definition
   addTouchedAddresses :: "machine_word set \<Rightarrow> unit machine_monad"
-  where "addTouchedAddresses da \<equiv> modify (\<lambda>s. s\<lparr>touched_addresses := da \<union> touched_addresses s\<rparr>)"
+  where "addTouchedAddresses da \<equiv> modify (touched_addresses_update ((\<union>) da))"
 
 text \<open>This instruction is required in the simulator, only.\<close>
 definition storeWordVM :: "machine_word \<Rightarrow> machine_word \<Rightarrow> unit machine_monad"
